<?xml version="1.0" encoding="UTF-8"?>

<section xml:id="sec-matrix-add-and-scale" xmlns:xi="http://www.w3.org/2001/XInclude">
  <title>Matrix addition and scalar multiplication</title>

 <definition xml:id="def-matrix-sum">
<statement>
<p>
The <term>sum</term> of two <m>m\times n</m> matrices
<me>
A = [a_{ij}]_{m\times n}, \qquad B = [b_{ij}]_{m\times n}
</me>
is the <m>m\times n</m> matrix
<me>
A + B  = [a_{ij} + b_{ij}]_{m\times n}
</me>.
</p>
</statement>
</definition>

<p>
So to add matrices, we add each component. Note that the matrices are required to be the same size. 
Scalar multiplication of matrices is also defined by considering each component.
</p>


<definition xml:id="def-scalar-multiple">
<title>Scalar multiple</title>
<statement>
<p>
The <term>scalar multiple</term> of an <m>m\times n</m> matrix <m>A = [a_{ij}]_{m\times n}</m> by a 
scalar <m>c \in \R</m> is the <m>m \times n</m> matrix
<me>
cA = [ca_{ij}]_{m\times n}
</me>.
</p>
</statement>
</definition>

<p>
Like for vectors (and for numbers), we write <m>-A = (-1)A</m> and <m>A - B = A + (-B)</m>.
</p>

<example xml:id="ex-matrix-algebra-basic">
<statement>
<p>
Let
<me>
A =
\begin{bmatrix}
  2 \amp  3  \amp  1 \\
  0 \amp  -1 \amp  2 \\
  5 \amp  0  \amp  3
\end{bmatrix}
, \qquad B =
\begin{bmatrix}
  1 \amp  2 \\
  3 \amp  4
\end{bmatrix}
, \qquad C =
\begin{bmatrix}
  -1 \amp  0 \amp  7 \\
  5  \amp  2 \amp  3 \\
  1  \amp  0 \amp  0
\end{bmatrix}

</me>. Find all of the following that are defined: <m>2A + 3C</m>, <m>A-C</m>, <m>A+B</m>, <m>B+C</m>.
</p>
<p>We calculate that
<md>
<mrow>
2A + 3C \amp  = 2
\begin{bmatrix}
  2 \amp  3  \amp  1 \\
  0 \amp  -1 \amp  2 \\
  5 \amp  0  \amp  3
\end{bmatrix}
+ 3
\begin{bmatrix}
  -1 \amp  0 \amp  7 \\
  5  \amp  2 \amp  3 \\
  1  \amp  0 \amp  0
\end{bmatrix}\\
\amp =
\begin{bmatrix}
  4  \amp  6  \amp  2 \\
  0  \amp  -2 \amp  4 \\
  10 \amp  0  \amp  6
\end{bmatrix}
+
\begin{bmatrix}
  -3 \amp  0 \amp  21 \\
  15 \amp  6 \amp  9  \\
  3  \amp  0 \amp  0
\end{bmatrix}
\\
\amp  =
\begin{bmatrix}
  1  \amp  6 \amp  23 \\
  15 \amp  4 \amp  13 \\
  13 \amp  0 \amp  6
\end{bmatrix}
</mrow>
</md>
and
<me>
A-C =
\begin{bmatrix}
  2 \amp  3  \amp  1 \\
  0 \amp  -1 \amp  2 \\
  5 \amp  0  \amp  3
\end{bmatrix}
-
\begin{bmatrix}
  -1 \amp  0 \amp  7 \\
  5  \amp  2 \amp  3 \\
  1  \amp  0 \amp  0
\end{bmatrix}
=
\begin{bmatrix}
  3  \amp  3  \amp  -6 \\
  -5 \amp  -3 \amp  -1 \\
  4  \amp  0  \amp  3
\end{bmatrix}
</me>.
<m>A+B</m> and <m>B+C</m> are not defined, since <m>B</m> is a different size to <m>A</m> and <m>C</m>.
</p>
</statement>
</example>

<p>
Matrix addition and scalar multiplication has the following properties.
</p>

<theorem xml:id="thm-matrix-addition">
<statement>
<p>
Let <m>A, B, C</m> be <m>m\times n</m> matrices, and let <m>r, s</m> be scalars. Then
<ol>
<li>
<p><m>A + B=B +A\quad</m> (commutativity of addition)
</p>
</li>
<li>
<p><m>(A+B)+C = A+(B+C)\quad</m> (associativity)
</p>
</li>
<li>
<p><m>A + 0_{m\times n} = A</m>
</p>
</li>
<li>
<p><m>A+(-A) = 0_{m\times n}</m>
</p>
</li>
<li>
<p><m>r(A+B) = rA +rB\quad</m> (distributivity)
</p>
</li>
<li>
<p><m>(r+s)A = rA + sA\quad</m> (distributivity)
</p>
</li>
<li>
<p><m>r(sA) = (rs)A</m>
</p>
</li>
<li>
<p><m>1A = A</m>.</p>
</li>
</ol>
</p>
</statement>
</theorem>

<!--<exercise>
<statement>
\label{prob: matrix addition}
<p>Prove <xref ref="thm-matrix addition"/>, or at least think about why it should be true.</p>
</statement>
<hint>
</hint>
<answer>
</answer>
<solution>
</solution>
</exercise>-->

<p>
Notice that these are the same properties satisfied for vector addition and scalar multiplication 
(see <xref ref="thm-vec-prop"/>).
</p>

</section>