<?xml version="1.0" encoding="UTF-8"?>

<section xml:id="sec-row-and-column-spaces" xmlns:xi="http://www.w3.org/2001/XInclude">
  <title>Row, column and null spaces</title>

<p>
Suppose <m>A</m> is an <m>m\times n</m> matrix. There are three subspaces we associate 
to <m>A</m>. 
</p>

<definition xml:id="def-row-and-col-spaces">
<statement>
<p>
<ul>

  <li>
  <p> 
  The <term>row space</term> of <m>A</m>, denoted <m>\operatorname{row}(A)</m>, is the subset
  of <m>\R^n</m> that is spanned by the rows of <m>A</m> (considered as vectors).
  </p>
  </li>
  
  <li>
  <p> 
  The <term>column space</term> of <m>A</m>, denoted <m>\operatorname{col}(A)</m>, is the subset
  of <m>\R^m</m> that is spanned by the columns of <m>A</m> (considered as vectors).
  </p>
  </li>
  
</ul>
</p>
</statement>
</definition>

<remark xml:id="rem-row-and-sol-spaces">
<statement>
<p>
<ul>

  <li>
  <p> 
  We know from <xref ref="thm-spans-are-subspaces"/> that the row and column 
  spaces of a matrix are subspaces. 
  </p>
  </li>
  
  <li>
  <p> 
  Be careful to note that 
  <ul>

  <li>
  <p> 
  <m>\operatorname{row}(A)</m> is a subspace of <m>\R^{\#\text{ of columns of }A}</m>
  </p>
  </li>
  
  <li>
  <p> 
  <m>\operatorname{col}(A)</m> is a subspace of <m>\R^{\#\text{ of rows of }A}</m>.
  </p>
  </li>
  
</ul>
  </p>
  </li>
  
</ul>
</p>
</statement>
</remark>

<p>
The third subspace we associate to a matrix is defined a little differently.
</p>

<definition xml:id="def-null-space">
<statement>
<p>
The <term>null space</term> of <m>A</m>, denoted <m>\operatorname{null}(A)</m>, is the subset
<md>
\operatorname{null}(A) := \{\vect{x}\in \R^n : A\vect{x}=\vect{0}\}\subseteq \R^n.
</md>
</p>
</statement>
</definition>


<theorem xml:id="thm-null-space-is-subspace">
<statement>
<p>
If <m>A</m> is <m>m\times n</m>, then <m>\operatorname{null}(A)</m> is a subspace of <m>\R^n</m>.
</p>
</statement>

<proof>
<p>
We have <m>A\vect{0}=\vect{0}\implies \vect{0}\in\operatorname{null}(A)</m>.
</p>

<p>
Let <m>\vect{x},\vect{y}\in \operatorname{null}(A)</m>. Then
<md>
A(\vect{x}+\vect{y})=A\vect{x}+A\vect{y}=\vect{0}+\vect{0}=\vect{0},
</md>
and hence <m>\vect{x}+\vect{y}\in\operatorname{null}(A)</m>.
</p>

<p>
Let <m>\vect{x}\in \operatorname{null}(A)</m> and <m>c\in\R</m>. Then
<md>
A(c\vect{x})=cA\vect{x}=c\vect{0}=\vect{0},
</md>
and hence <m>c\vect{x}\in\operatorname{null}(A)</m>.
</p>
</proof>
</theorem>

<definition xml:id="def-finding-null-space">
<statement>
<p>
Find the null space of 
<md>
A=\begin{bmatrix} 2 \amp 3 \amp 1\\ 0 \amp -1 \amp 1\end{bmatrix}.
</md>
</p>

<p>
We want <m>\vect{x}=\begin{bmatrix}x\\y\\z\end{bmatrix}</m> such that <m>A\vect{x}=\vect{0}</m>.
</p>

<p> The augmented matrix is 
<md>
\begin{amatrix}{ccc}2\amp 3\amp 1\amp 0\\0\amp -1\amp 1\amp 0\end{amatrix},
</md>
which is already in REF!
</p>
<p>
Let <m>z=t</m>, <m>t\in\R</m>. Then 
<md>
-y+z=0\implies y=z\implies y=t,
</md>
and
<md>
2x+3y+z=0\implies 2x+3t+t=0\implies x=-2t.
</md>
So
<md>
\operatorname{null}(A)=\left\{\begin{bmatrix}-2t\\t\\t\end{bmatrix} : t\in\R\right\}
=\lspan\left(\begin{bmatrix}-2\\1\\1\end{bmatrix}\right)
</md>
is the line through the origin with direction vector <m>[-2,1,1]</m>.
</p>
</statement>
</definition>

</section>