<?xml version="1.0" encoding="UTF-8"?>

<section xml:id="sec-properties-of-inverses" xmlns:xi="http://www.w3.org/2001/XInclude">
  <title>Properties of inverses</title>

 <p>
Let <m>a, b, x \in \R</m> and consider the equation of real numbers
<me>
ax = b
</me>.
If <m>a\ne 0</m>, then <m>a</m> has the inverse <m>a\inv = 1/a</m>, and there is a unique solution
<me>
x = a\inv b = \frac{1}{a}b = \frac{b}{a}
</me>.
This works because
<md>
<mrow>
ax = b \amp  \implies a\inv a x = a\inv b \\
\amp  \implies 1x = x = a\inv b
</mrow>
</md>.
</p>

<p>
We see that the key property of <m>a\inv</m> is that <m>a\inv a = 1</m>, and similarly it's useful 
that <m>a\inv a = 1</m>. (For real numbers this is essentially the same thing, because multiplication 
is commutative, but remember that matrix multiplication is not commutative.) We will define matrix 
inverses to have these properties, so that we can likewise solve the matrix equation <m>AX = B</m> 
to get <m>X = A\inv B</m>.
</p>


<definition xml:id="def-inverse">
<statement>
<p>
An <term>inverse</term> of an <m>n\times n</m> matrix <m>A</m> is an <m>n\times n</m> matrix <m>B</m> 
such that
<me>
AB = BA = I_n
</me>.
If such a matrix <m>B</m> exists, then we say that <m>A</m> is <term>invertible</term>.
</p>
</statement>
</definition>

<p>
Note that we require <m>A</m> and <m>B</m> to both be <m>n\times n</m> so that <m>AB</m> and <m>BA</m> 
are both defined.
</p>

<example xml:id="ex-inverse-check">
<statement>
<p>
Let
<me>
A =
\begin{bmatrix}
  2 \amp  5 \\ 1\amp  3
\end{bmatrix}
, \qquad B =
\begin{bmatrix}
  3 \amp  -5 \\ -1 \amp  2
\end{bmatrix}
</me>.
Then
<md>
<mrow>
AB \amp  =
\begin{bmatrix}
  2 \amp  5 \\ 1\amp  3
\end{bmatrix}
\begin{bmatrix}
  3 \amp  -5 \\ -1 \amp  2
\end{bmatrix}
=
\begin{bmatrix}
  1 \amp  0 \\ 0 \amp  1
\end{bmatrix}
= I_2, \\
BA \amp  =
\begin{bmatrix}
  3 \amp  -5 \\ -1 \amp  2
\end{bmatrix}
\begin{bmatrix}
  2 \amp  5 \\ 1\amp  3
\end{bmatrix}
=
\begin{bmatrix}
  1 \amp  0 \\ 0 \amp  1
\end{bmatrix}
= I_2
</mrow>
</md>.
So by definition, <m>B</m> is an inverse of <m>A</m> (and <m>A</m> is an inverse of <m>B</m>).
</p>
</statement>
</example>

<p>
The zero matrix is not invertible since for any matrix <m>B</m>, we have <m>0B = B0 = 0 \ne I_n</m>. 
However, unlike real numbers, there are nonzero matrices which are not invertible.
</p>


<example xml:id="ex-non-invertible">
<statement>
<p>
Let
<me>
A =
\begin{bmatrix}
  1 \amp  -1 \\ -2 \amp  2
\end{bmatrix}
, \qquad B =
\begin{bmatrix}
  a \amp  b \\ c\amp  d
\end{bmatrix}
</me>.
Calculate <m>AB</m> and show that <m>A</m> is not invertible.
</p>
<p>
We have
<md>
<mrow>
AB \amp  =
\begin{bmatrix}
  1 \amp  -1 \\ -2 \amp  2
\end{bmatrix}
\begin{bmatrix}
  a \amp  b \\ c\amp  d
\end{bmatrix}
\\
\amp  =
\begin{bmatrix}
  a-c \amp  b-d \\ -2a+2c\amp  -2(b-d)
\end{bmatrix}
</mrow>
</md>.
If the <m>(1, 2)</m>-entry is zero, then the <m>(2, 2)</m>-entry is also zero, so is not equal to 1. 
This shows that
<me>
AB \ne I_2 =
\begin{bmatrix}
  1 \amp  0 \\
  0 \amp  1
\end{bmatrix}
,
</me>
regardless of the value of <m>a, b, c, d\in \R</m>. Therefore <m>A</m> has no inverse.
</p>
</statement>
</example>

<theorem xml:id="thm-unique">
<statement>
<p>
If an <m>n\times n</m> matrix <m>A</m> is invertible, then it has a unique inverse.
</p>
</statement>

<proof>
<p>
Suppose <m>B</m> and <m>C</m> are any two inverses of <m>A</m>. Then
<me>
B = BI = B(AC)
</me>
since <m>C</m> is an inverse of <m>A</m>. But then
<me>
B(AC) = (BA)C = IC = C
</me>
using associativity and that <m>B</m> is an inverse of <m>A</m>. Thus <m>B=C</m>.
</p>
</proof>
</theorem>

<p>
Since if <m>A</m> is invertible it only has one inverse, we will now refer to it as the inverse of 
<m>A</m>, and denote it by <m>A\inv</m>.
</p>


<remark xml:id="rem-inverse-notation">
<title></title>
<p>Do not write <m>1/A</m> for the inverse <m>A\inv</m>. This is a number divided by a matrix, 
so it makes no sense. Therefore, if we have a matrix equation <m>AX = B</m> where <m>A</m> is 
invertible, and solve it to get <m>X = A\inv B</m>, you should think of this as multiplication 
by <m>A\inv</m> rather than division by <m>A</m>. Even though for real numbers this is the same 
thing, to avoid confusion it is best to never think about division when working with matrices.
</p>
</remark>

<p>
Matrix inversion has the following properties, which are similar to the properties for the matrix 
transpose.</p>

<theorem xml:id="thm-inv">
<statement>
<p>Suppose <m>A</m> and <m>B</m> are invertible <m>n\times n</m> matrices, and <m>c\in \R</m> is a nonzero scalar. Then
<ol>
<li>
<p><m>A\inv</m> is invertible, and <m>(A\inv)\inv = A</m>
</p>
</li>
<li>
<p><m>cA</m> is invertible, and <m>(cA)\inv = \frac{1}{c}A\inv</m>
</p>
</li>
<li>
<p><m>AB</m> is invertible, and <m>(AB)\inv = B\inv A\inv</m>
</p>
</li>
<li>
<p><m>A^T</m> is invertible, and <m>(A^T)\inv = (A\inv)^T</m>
</p>
</li>
<li>
<p><m>A^k</m> is invertible for any <m>k \in \N</m>, and <m>(A^k)\inv = (A\inv)^k</m>.</p>
</li>
</ol></p>
</statement>
</theorem>

<p>
We will prove the first 4 properties. The proof of Property 5 is an exercise.
</p>

<proof>
<p>
The equation <m>AA\inv = A\inv A = I_n</m> which comes from <m>A</m> being invertible also says 
that <m>A\inv</m> is invertible and <m>(A\inv)\inv = A</m> (think about this) which proves 1. 
Property 2 follows from the calculation
<md>
<mrow>
cA\biggl(\frac{1}{c}A\inv\biggr) \amp  = c\frac{1}{c}AA\inv = 1I = I   \\
\biggl(\frac{1}{c}A\inv\biggr)cA \amp  = \frac{1}{c}c A\inv A = 1I = I
</mrow>
</md>
and Property 3 follows from the calculation
<md>
<mrow>
AB(B\inv A\inv) \amp  = A(B B\inv)A\inv = AA\inv = I    \\
(B\inv A\inv)AB \amp  = B\inv (A\inv A)B = B\inv B = I
</mrow>
</md>.
For Property 4, observe that
<md>
<mrow>
A^T(A\inv)^T  \amp  = (A\inv A)^T = I^T = I         \\
(A\inv)^T A^T \amp  = (AA\inv)^T = I^T = I.
</mrow>
</md>
</p>
</proof>

<p>
We will use the notation <m>A^{-k} = (A\inv)^k</m>.
</p>

<example xml:id="ex-matrix-algebra-with-inverses">
<statement>
<p>Solve <m>A\inv (BX)\inv = (A\inv B^3)^2</m> for <m>X</m> in terms of <m>A</m> and <m>B</m>.</p>
<p>We calculate, using properties of the matrix inverse, that
<md>
<mrow>
A\inv (BX)\inv \amp = (A\inv B^3)^2 \\
\amp  \implies AA\inv(BX)\inv = A(A\inv B^3)^2                        \\
\amp  \implies (BX)\inv = A(A\inv B^3)^2                              \\
\amp  \implies ((BX)\inv)\inv = (A(A\inv B^3)^2)\inv                  \\
\amp  \implies BX = (A\inv B^3)^{-2} A\inv                            \\ \amp  \implies B\inv BX = B\inv (A\inv B^3)^{-2} A\inv\\
\amp  \implies X = B\inv(B^{-3}A)^2 A\inv = B\inv B^{-3}AB^{-3}AA\inv \\
\amp  \implies X = B^{-4}AB^{-3}.
</mrow>
</md>
</p>
</statement>
</example>



</section>