<?xml version="1.0" encoding="UTF-8"?>

<section xml:id="sec-dot-products" xmlns:xi="http://www.w3.org/2001/XInclude">
  <title>Dot products</title>

<definition xml:id="def-dot-product">
  <title>(Dot product)</title>
  
  
<statement>
<p>The <term>dot product</term> of the vectors <m>\vect{u} = [u_1, u_2, \dots, u_n]</m> and 
<m>\vect{v} = [v_1, v_2, \dots, v_n] \in \R^n</m> is the scalar
<me>
\vect{u}\cdot\vect{v}= u_1 v_1 + u_2v_2 + \cdots + u_n v_n
</me>.
</p>
</statement>
</definition>

<p>
It is important not to leave out the dot when writing the dot product, to distinguish this from the cross 
product which will be introduced later. For example, if <m>\vect{u} = [1, 3]</m> and <m>\vect{v} = [2, -4]</m>, 
then
<me>
\vect{u}\cdot\vect{v} = 1(2) + 3(-4) = 2-12 = -10
</me>.
If <m>\vect{u} = [2, -1, 0]</m> and <m>\vect{v} = [1, 4, 9]</m>, then
<me>
\vect{u}\cdot\vect{v} = 2(1) + (-1)4 + 0(9) = 2-4+0 = -2
</me>.
</p>

<p>
The dot product has the following properties.
</p>

<theorem xml:id="thm-props-dot-product">
  <title>(Properties of the dot product)</title>
  
  
<statement>
<p>Let <m>\vect{u}, \vect{v}, \vect{w} \in \R^n</m>, and <m>c \in \R</m>. Then
<ol>
<li>
<p><m>\vect{u} \cdot\vect{v} = \vect{v} \cdot\vect{u}\quad </m> (commutativity)
</p>
</li>
<li>
<p><m>\vect{u}\cdot (\vect{v}+\vect{w}) = \vect{u}\cdot \vect{v} + \vect{u} \cdot \vect{w}\quad</m> (distributivity)
</p>
</li>
<li>
<p><m>(c\vect{u})\cdot\vect{v} = c(\vect{u}\cdot\vect{v})</m>
</p>
</li>
<li>
<p><m>\vect{u}\cdot \vect{u} \ge 0</m>, with equality if and only if <m>\vect{u} = 0\quad</m> (positive-definiteness)
</p>
</li>
<li>
<p><m>\|\vect{u}\| = \sqrt{\vect{u}\cdot\vect{u}}</m>
</p>
</li>
<li>
<p><m>|\vect{u}\cdot\vect{v}| \le \|\vect{u}\|\|\vect{v}\|\quad</m> (Cauchy&#x2013;Schwarz inequality)
</p>
</li>
<li>
<p><m>\|\vect{u} + \vect{v}\| \le \|\vect{u}\| + \|\vect{v}\|\quad</m> (triangle inequality)
</p>
</li>
</ol></p>
</statement>
</theorem>

<p>
We prove Properties 4-7.
</p>

<proof>
<p>
Let <m>\vect{u} = [u_1, u_2, \dots, u_n] \in \R^n</m>. Observe that
<me>
\vect{u} \cdot \vect{u} = u_1^2 + u_2^2 + \dots +u_n^2
</me>.
We see that this is the square of <m>\|\vect{u}\|</m>, proving Property 5, and it is a sum of squared real 
numbers. Therefore <m>\vect{u} \cdot \vect{u} \ge 0</m>, and it equals zero if and only if 
<m>u_1 = u_2 = \cdots = u_n = 0</m>, i.e. if and only if <m>\vect{u} = \vect{0}</m>, proving Property 4.
</p>

<p>
Now consider Property 6. If <m>\vect{u}=\vect{0}</m> or <m>\vect{v} = \vect{0}</m>, then both sides are zero 
and the inequality is true. Therefore, suppose one of them is nonzero, say <m>\vect{v} \ne \vect{0}</m>. 
We first calculate that
<md>
<mrow>
0 \le \|\vect{u} -c\vect{v}\|^2 \amp  = (\vect{u} -c\vect{v})\cdot (\vect{u} -c\vect{v})                                                        \\
\amp  = \vect{u}\cdot (\vect{u} - c\vect{v}) - c\vect{v}\cdot (\vect{u} - c\vect{v})                            \\
\amp  = \vect{u}\cdot \vect{u} - c\vect{u}\cdot \vect{v} - c\vect{v} \cdot \vect{u} + c^2 \vect{v}\cdot\vect{v} \\
\amp  = \|\vect{u}\|^2 - 2c\vect{u}\cdot \vect{v} + c^2\|\vect{v}\|^2
</mrow>
</md>.
</p>

<p>
Applying this with <m>c = \frac{\vect{u}\cdot \vect{v}}{\|\vect{v}\|^2}</m>, we get
<md>
<mrow>
0 \le \left|\vect{u} - \left(\frac{\vect{u}\cdot \vect{v}}{\|\vect{v}\|^2}\right)\right|^2 \amp  = \|\vect{u}\|^2 - 2\left(\frac{\vect{u}\cdot \vect{v}}{\|\vect{v}\|^2}\right)\vect{u}\cdot \vect{v} + \left(\frac{\vect{u}\cdot \vect{v}}{\|\vect{v}\|^2}\right)^2\|\vect{v}\|^2 \\
\amp  =\|\vect{u}\|^2 - \frac{(\vect{u}\cdot\vect{v})^2}{\|\vect{v}\|^2}
</mrow>
</md>.
</p>

<p>
Therefore <m>\frac{(\vect{u}\cdot\vect{v})^2}{\|\vect{v}\|^2} \le \|\vect{u}\|^2</m>, which rearranges to 
give <m>(\vect{u}\cdot\vect{v})^2 \le \|\vect{u}\|^2\|\vect{v}\|^2</m>. Taking square roots, 
<m>|\vect{u}\cdot\vect{v}| \le \|\vect{u}\|\|\vect{v}\|</m>, which proves the Cauchy&#x2013;Schwarz inequality.
</p>

<p>
For Property 7, both sides of the inequality are nonnegative, so it is equivalent to show that
<me>
\|\vect{u}+\vect{v}\|^2 \le (\|\vect{u}\| + \|\vect{v}\|)^2
</me>.
Taking <m>c = -1</m> in the first calculation during the proof of Property 6, we get
<md>
<mrow>
\|\vect{u} + \vect{v}\|^2 \amp  = \|\vect{u} - (-1)\vect{v}\|^2                                        \\
\amp  = \|\vect{u}\|^2 - 2(-1)\vect{u}\cdot \vect{v} + (-1)^2 \|\vect{v}\|^2 \\
\amp  =  \|\vect{u}\|^2 +2\vect{u}\cdot \vect{v} + \|\vect{v}\|^2            \\
\amp  \le \|\vect{u}\|^2 + 2 \|\vect{u}\|\|\vect{v}\| + \|\vect{v}\|^2       \\
\amp  = (\|\vect{u}\| + \|\vect{v}\|)^2
</mrow>
</md>,
where in the second-last line we used the Cauchy&#x2013;Schwarz inequality. This proves the triangle inequality.
</p>
</proof>

<p>
Geometrically, consider the triangle formed by the vectors <m>\vect{a}, \vect{b}</m> and <m>\vect{a+b}</m>. 
Because the length of any side of a triangle is less than or equal to the sum of the the other lengths, 
we have <m>\|\vect{a}+\vect{b}\| \le \|\vect{a}\| + \|\vect{b}\|</m>. This explains the name of the 
inequality.
</p>

<figure xml:id="triangle-inequality">
<caption>The triangle inequality</caption>
<image width="60%">
<latex-image>
\begin{tikzpicture}[scale = 3.6]
    %x-y axis
    \draw (0, 0) node [anchor = north east] {$O$};
    \draw [vector,->] (-0.375, 0) -- (1.05,0) node [right] {$x$};
    \draw [vector,->] (0, -0.375) -- (0,1.05) node [above] {$y$};

    %arrows
    \draw [vector,->, red] (0, 0) -- (0.6, 0.3);
    \draw [vector,->, blue] (0.6, 0.3) -- (0.8, 0.8);
    \draw [vector,->, violet] (0, 0) -- (0.79, 0.79);

    %labels
    \draw (0.37, 0.2) node [below, red] {$\vect{a}$};
    \draw (0.7, 0.5) node [right, blue] {$\vect{b}$};
    \draw (0.44, 0.5) node [left, violet] {$\vect{a} + \mathbf{b}$};
\end{tikzpicture}
</latex-image>
</image>
</figure>



</section>