<?xml version="1.0" encoding="UTF-8"?>

<section xml:id="sec-cross-products" xmlns:xi="http://www.w3.org/2001/XInclude">
  <title>Cross products</title>

 <p>
The cross product is another operation on vectors. It is only defined for vectors in <m>\R^3</m>, and its 
output is another vector in <m>\R^3</m>.
</p>


<definition xml:id="def-cross-product">
  <title>(Cross product)</title>
  
  
<statement>
<p>
The <term>cross product</term> of the vectors <m>\vect{u}=[u_1, u_2, u_3], \vect{v} = [v_1, v_2, v_3] \in \R^3</m>
is the vector
<me>
\vect{u}\times\vect{v} = [u_2v_3 - u_3v_2, u_3v_1 - u_1v_3, u_1v_2-u_2v_1]
</me>.
</p>
</statement>
</definition>

<p>
To help remember the formula, we can use the array method (<xref ref="fig-braid"/>). It involves 3 pairs of 
lines, one for each component of the resulting vector. Starting at <m>u_2</m>, multiply the components 
connected by the solid line, then subtract the product of the components connected by the dashed line. 
For example, the first component is <me>
\text{first solid line} - \text{first dashed line} = u_2v_3 - v_2u_3,
</me>
and so on for the rest.
</p>

<figure xml:id="fig-braid">
<caption>Diagram for the array method</caption>
<image width="60%">
<latex-image>
\begin{tikzcd}
  {u_1} \amp {u_2} \amp {u_3} \amp {u_1} \amp {u_2} \amp {u_3} \amp {} \\
  {v_1} \amp {v_2} \amp {v_3} \amp {v_1} \amp {v_2} \amp {v_3} \amp {}
    \arrow[no head, from=1-2, to=2-3]
    \arrow[no head, from=1-3, to=2-4]
    \arrow[no head, from=1-4, to=2-5]
    \arrow[dashed, no head, from=2-2, to=1-3]
    \arrow[dashed, no head, from=2-3, to=1-4]
    \arrow[dashed, no head, from=2-4, to=1-5]
\end{tikzcd}
</latex-image>
</image>
</figure>



<p>
Alternatively, to notice the `criss-cross' pattern it helps to write the vectors using columns:
<me>
\begin{bmatrix}
  u_1 \\ u_2\\ u_3
\end{bmatrix}
\times
\begin{bmatrix}
  v_1 \\ v_2\\ v_3
\end{bmatrix}
=
\begin{bmatrix}
  u_2v_3 - u_3v_2 \\ u_3v_1 - u_1v_3\\ u_1v_2-u_2v_1
\end{bmatrix}
</me>.
</p>

<p>
Here are three examples which also showcase properties of the cross product.
</p>


<example xml:id="ex-cross">
<statement>
<p>
If <m>\vect{u} = [3, 1, 2]</m> and <m>\vect{v} = [5, 0, 4]</m>, then
<me>
\vect{u} \times \vect{v} = [1(4) - 2(0), 2(5) - 3(4), 3(0) - 1(5)] = [4, -2, -5]
</me>
and
<me>
\vect{v}\times\vect{u} = [0(2) - 4(1), 4(3) - 5(2), 5(1) - 0(3)] = [-4, 2, 5]
</me>.
Notice that <m>\vect{u} \times \vect{v} = - \vect{v} \times \vect{u}</m>.
</p>
</statement>
</example>

<figure xml:id="fig-braid_ex">
<caption>Array method for <m>\vect{u} \times \vect{v}</m> from <xref ref="ex-cross"/></caption>
<image width="60%">
<latex-image>
<md>
\begin{tikzcd}
	{3} \amp {1} \amp {2} \amp {3} \amp {1} \amp {2} \\
	{5} \amp {0} \amp {4} \amp {5} \amp {0} \amp {4}
	\arrow[no head, from=1-2, to=2-3]
	\arrow[no head, from=1-3, to=2-4]
	\arrow[no head, from=1-4, to=2-5]
	\arrow[dashed, no head, from=2-2, to=1-3]
	\arrow[dashed, no head, from=2-3, to=1-4]
	\arrow[dashed, no head, from=2-4, to=1-5]
\end{tikzcd}
</md>
</latex-image>
</image>
</figure>

<example xml:id="ex-dot-and-cross">
  <title>(Finding cross product)</title>
  
  
<statement>
<p>
Find <m>\vect{u}\cdot (\vect{u}\times\vect{v})</m> and <m>\vect{v}\cdot (\vect{u}\times\vect{v})</m> 
for <m>\vect{u} = [3, 1, 2]</m> and <m>\vect{v} = [5, 0, 4]</m>. 
</p>
</statement>
<solution>
  <p>
  From the previous example, we know 
<m>\vect{u} \times\vect{v} = [4, -2, -5]</m>. So
<me>
\vect{u}\cdot(\vect{u}\times\vect{v}) = [3, 1, 2] \cdot [4, -2, -5] = 12-2-10 = 0,
</me>
<me>
\vect{v}\cdot (\vect{u}\times\vect{v}) = [5, 0, 4] \cdot [4, -2, -5] = 20+0-20 = 0.
</me>
</p>
</solution>
</example>

<example xml:id="ex-uxuiszero">
<statement>
<p>If <m>\vect{u} = [3, 1, 2]</m>, then
<me>
\vect{u}\times \vect{u} = [2-2, 6-6, 3-3] = [0, 0, 0] = \vect{0}.
</me></p>
</statement>
</example>

<p>
The next theorem lists the main properties of the cross product.
</p>


<theorem xml:id="thm-cross-product-props">
  <title>(Properties of cross products)</title>
  
  
<statement>
<p>
Let <m>\vect{u}, \vect{v}, \vect{w} \in\R^3</m> and <m>c\in \R</m>. Then
<ol>
<li>
<p><m>\vect{u} \times \vect{v} = -\vect{v} \times \vect{u}\quad</m> (anti-commutativity)
</p>
</li>
<li>
<p><m>\vect{u} \cdot (\vect{u}\times \vect{v}) = \vect{v} \cdot(\vect{u}\times \vect{v} ) = 0</m>
</p>
</li>
<li>
<p><m>\vect{u} \times \vect{u} = \vect{0}</m>
</p>
</li>
<li>
<p><m>\vect{u} \times \vect{0} = \vect{0} \times\vect{u} = \vect{0}</m>
</p>
</li>
<li>
<p><m>\vect{u}\times (\vect{v} + \vect{w})=\vect{u}\times \vect{v} + \vect{u} \times \vect{w}\quad</m> (left distributivity)
</p>
</li>
<li>
<p><m>(\vect{u} + \vect{v})\times \vect{w} = \vect{u} \times\vect{w} + \vect{v} \times \vect{w}\quad</m> (right distributivity)
</p>
</li>
<li>
<p><m>(c\vect{u})\times \vect{v} = \vect{u} \times (c\vect{v}) = c(\vect{u}\times \vect{v})</m>.</p>
</li>
</ol>
</p>
</statement>
</theorem>

<p>
Property 2 says that <m>\vect{u} \times \vect{v}</m> is orthogonal to <m>\vect{u}</m> and <m>\vect{v}</m>. 
We will prove Properties 2, 3, and 5.
</p>

<proof>
<p>
Let <m>\vect{u} = [u_1, u_2, u_3], \vect{v} = [v_1, v_2, v_3]</m> and <m>\vect{w} = [w_1, w_2, w_3]</m>. 
Property 2 holds since
<md>
<mrow>
\vect{u} \cdot (\vect{u}\times \vect{v}) \amp  = [u_1, u_2, u_3]\cdot [u_2v_3 - u_3v_2, u_3v_1 - u_1v_3, u_1v_2-u_2v_1] \\
\amp  = u_1u_2v_3 - u_1u_3v_2 + u_2u_3v_1 - u_2u_1v_3 + u_3u_1v_2 - u_3u_2v_1  \\
\amp  =0;
</mrow>
</md>
the calculation that <m>\vect{v} \cdot(\vect{u}\times \vect{v}) = 0</m> is similar. We can deduce Property 3 
from Property 1 by observing that
<me>
\vect{u} \times \vect{u} = -\vect{u} \times \vect{u},
</me>
so <m>\vect{u} \times \vect{u} = 0</m>. Finally, the proof of Property 5 is that
<md>
<mrow>
\amp\vect{u}\times (\vect{v} + \vect{w}) \\
\amp  = [u_1, u_2, u_3]\times [v_1 + w_1, v_2 + w_2, v_3 + w_3]                                                   \\
\amp  = [u_2(v_3 + w_3) - u_3(v_2 + w_2), u_3(v_1 + w_1)- u_1(v_3 + w_3), \\
\amp\qquad\qquad u_1(v_2 + w_2) - u_2(v_1 + w_1)]       \\
\amp  = [u_2v_3 - u_3v_2, u_3v_1 - u_1v_3, u_1v_2 - u_2v_1] \\
\amp\quad\qquad+ [u_2w_3 - u_3w_2, u_3w_1 - u_1w_3, u_1w_2 - u_2w_1] \\
\amp  = \vect{u} \times \vect{v} + \vect{u} \times \vect{w}.
</mrow>
</md>
</p>
</proof>

<p>
Importantly, the cross product is not associative! This means that, for 
<m>\vect{u}, \vect{v}, \vect{w} \in \R^3</m>,
<me>
(\vect{u}\times \vect{v})\times \vect{w} \ne \vect{u} \times (\vect{v}\times \vect{w})
</me>.
For example, if <m>\vect{u} = [1, 1, 0], \vect{v} = [0, 1, 1], \vect{w} = [0, 0, 1]</m>, then
<me>
(\vect{u}\times \vect{v})\times \vect{w} = [1, -1, 1] \times [0, 0, 1] =[-1, -1, 0]
</me>
while
<me>
\vect{u} \times (\vect{v}\times \vect{w}) = [1, 1, 0] \times [1, 0, 0] = [0, 0, -1]
</me>.
</p>

<example xml:id="ex-cross-product-algebra">
  <title>(Simplifying a cross product)</title>
  
  
<statement>
<p>
Simplify <m>(\vect{u} + \vect{v}) \times (\vect{u} - \vect{v})</m> using the properties in the theorem.
</p>
</statement>
<solution>
  <p>
  We have
<md>
<mrow>
(\vect{u} + \vect{v}) \times (\vect{u} - \vect{v}) \amp  =  (\vect{u} + \vect{v}) \times \vect{u} + (\vect{u} + \vect{v}) \times (-\vect{v})\quad \text{(Property 5)} \\
\amp  = (\vect{u} + \vect{v}) \times \vect{u} - (\vect{u} + \vect{v})\times\vect{v}                               \quad \text{(Property 7)}           \\
\amp  = \vect{u}\times \vect{u} + \vect{v} \times \vect{u} - (\vect{u} \times \vect{v} + \vect{v}\times \vect{v}) \quad \text{(Property 6)}           \\
\amp  = \vect{v} \times \vect{u} - \vect{u} \times \vect{v}                                                       \quad \text{(Property 3)}        \\
\amp  = - 2\vect{u}\times \vect{v}.                                                                               \quad \text{(Property 1)} 
</mrow>
</md>
</p>
</solution>
</example>

<p>
Recall that <m>\vect{u} \times \vect{v}</m> is orthogonal to both <m>\vect{u}</m> and <m>\vect{v}</m>. 
If <m>\vect{u}</m> and <m>\vect{v}</m> are not parallel, then the set of linear combinations of 
<m>\vect{u}</m> and <m>\vect{v}</m> is a plane in <m>\R^3</m>. The cross product <m>\vect{u} \times \vect{v}</m> 
must be orthogonal to this plane, so there are only two choices for its direction. This is show in 
<xref ref="fig-plane_normals"/>: the two orthogonal vectors are the upwards normal vector and the 
downwards normal vector, drawn in red.
</p>



<!--<figure xml:id="fig-plane_normals">
<caption>There are two vectors which are orthogonal to the plane given by <m>\vect{u}</m> and <m>\vect{v}</m></caption>
plane_normals.tikz
</figure>-->

<figure xml:id="fig-plane_normals">
  <caption>There are two vectors which are orthogonal to the plane given by <m>\vect{u}</m> and <m>\vect{v}</m></caption>
  <image width="60%">
    <latex-image label="3d-plane">
\tdplotsetmaincoords{60}{120} % view angle for 3D plot
\begin{tikzpicture}[tdplot_main_coords, scale=0.65]
  % x-y plane
  \filldraw[fill=blue!20,opacity=0.5]
    (3,3,0) -- (-3,3,0) -- (-3,-3,0) -- (3,-3,0) -- cycle;

  % vectors
  \draw[very thick,->] (0,0,0) -- (2,0,0)
    node[xshift=-1.2mm,yshift=-1.2mm] {$\vect{u}$};
  \draw[very thick,->] (0,0,0) -- (0,2,0)
    node[xshift=1.2mm,yshift=-1.2mm] {$\vect{v}$};

  % normal vectors
  \fill[red] (0,0,0) circle (2pt);
  \draw[thick,->,red] (0,0,0) -- (0,0,4);
  \draw[thick,->,red] (0,0,0) -- (0,0,-4);
\end{tikzpicture}
    </latex-image>
  </image>
</figure>

<p>
  So the cross product can only point in one of two directions, but which one is it?
</p>

<assemblage xml:id="right-hand-rule">
  <title>(Right-hand rule)</title>
  <p>
The direction of <m>\vect{u} \times \vect{v}</m> is given by the right hand rule:
<ol>
<li>
<p>Point the fingers of your right hand straight in the direction of <m>\vect{u}</m>.</p>
</li>
<li>
<p>Curl fingers towards the direction of <m>\vect{v}</m>.</p>
</li>
<li>
<p>Your thumb points in the direction of <m>\vect{u}\times \vect{v}</m>.</p>
</li>
</ol>
</p>
<figure xml:id="fig-rhr">
<caption>The right hand rule</caption>
<!--RHR pic needed-->
</figure>
</assemblage>


<p>
Now that we know the direction of <m>\vect{u}\times \vect{v}</m>, we want to calculate its magnitude. 
First, it will help to have the following fact (we leave the proof as an exercise).
</p>


<assemblage xml:id="fact-length-of-cross">
<p>
Let <m>\vect{u}, \vect{v} \in \R^3</m>. Then we have
<md>
  \|\vect{u} \times\vect{v}\|^2 = \|\vect{u}\|^2\|\vect{v}\|^2 - |\vect{u}\cdot\vect{v}|^2
</md>.
</p>
</assemblage>

<p>
Now we can calculate the length of a cross product.
</p>


<theorem xml:id="Thm-lengpara">
  <title>(Length of cross product)</title>
  
  
<statement>
<p>
Let <m>\vect{u}, \vect{v} \in \R^3</m>, and <m>\theta</m> be the angle between <m>\vect{u}</m> and 
<m>\vect{v}</m> such that <m>0 \le \theta \le \pi</m>. Then
<me>
\|\vect{u} \times \vect{v}\| = \|\vect{u}\|\|\vect{v}\|\sin\theta
</me>.
</p>
</statement>

<proof>
<p>
By the boxed fact above and the geometric formula for the dot product,
<md>
<mrow>
\|\vect{u} \times\vect{v}\|^2 \amp  = \|\vect{u}\|^2\|\vect{v}\|^2 - |\vect{u}\cdot\vect{v}|^2              \\
\amp  = \|\vect{u}\|^2\|\vect{v}\|^2 - |\|\vect{u}\|\|\vect{v}\|\cos\theta|^2 \\
\amp  = \|\vect{u}\|^2\|\vect{v}\|^2(1-\cos^2\theta)                          \\
\amp  = \|\vect{u}\|^2\|\vect{v}\|^2\sin^2\theta
</mrow>
</md>.
Since <m>0 \le \theta\le \pi</m>, we have <m>\sin\theta \ge 0</m>, and so taking square roots gives the 
result.
</p>
</proof>
</theorem>

<example xml:id="ex-length-of-cross">
  <title>(Calculating length of cross product)</title>
  
  
<statement>
<p>
Suppose <m>\vect{u}, \vect{v} \in \R^3</m> are such that <m>\|\vect{u}\| = \sqrt{6}, \|\vect{v}\| = \sqrt{35}</m>, and 
<m>\vect{u}\cdot\vect{v} = 14</m>. Find <m>\|\vect{u} \times \vect{v}\|</m>.
</p>
</statement>
<solution>
  <p>
We first calculate that
<me>
\cos\theta = \frac{\vect{u}\cdot\vect{v}}{\|\vect{u}\|\|\vect{v}\|} = \frac{14}{\sqrt{6}\sqrt{35}} = \frac{14}{\sqrt{210}}
</me>.
Then <m>\sin^2\theta = 1- \cos^2\theta = \frac{1}{15}</m>, so <m>\sin\theta = \frac{1}{\sqrt{15}}</m>. (We used the 
  positive square root since <m>0\le\theta\le\pi</m>). Finally,
<me>
\|\vect{u} \times \vect{v}\| = \|\vect{u}\|\|\vect{v}\|\sin\theta = \sqrt{\frac{210}{15}} = \sqrt{14}.
</me>
</p>
</solution>
</example>



</section>